src/Util/BitVector.v
@@ -1,5 +1,5 @@
 From Coq Require Import Ascii Bvector NArith String.
-From HTTP2 Require Import Util.ByteVector.
+From HTTP2 Require Import Util.ByteVector Util.VectorUtil.
 Open Scope string_scope.
 
 Fixpoint pack {n : nat} (v : Bvector n) : string :=
@@ -21,6 +21,22 @@ Fixpoint Bvector_of_ByteVector {n : nat} (v : ByteVector n) : Bvector (n * 8) :=
   | [] => []
   | Ascii b0 b1 b2 b3 b4 b5 b6 b7::v' =>
     b0::b1::b2::b3::b4::b5::b6::b7::Bvector_of_ByteVector v'
+  end.
+
+Fixpoint ByteVector_of_Bvector {n : nat} : Bvector (n * 8) -> ByteVector n :=
+  match n with
+  | O => fun _ => []
+  | S n' =>
+    fun v =>
+      let (b0, v1) := Vector_uncons v in
+      let (b1, v2) := Vector_uncons v1 in
+      let (b2, v3) := Vector_uncons v2 in
+      let (b3, v4) := Vector_uncons v3 in
+      let (b4, v5) := Vector_uncons v4 in
+      let (b5, v6) := Vector_uncons v5 in
+      let (b6, v7) := Vector_uncons v6 in
+      let (b7, v8) := Vector_uncons v7 in
+      Ascii b0 b1 b2 b3 b4 b5 b6 b7::ByteVector_of_Bvector v8
   end.
 
 Fixpoint N_of_Bvector_rec {n : nat} (acc : N) (v : Bvector n) : N :=
